Updates

high2/Zeta.EAC.fsti
@@ -3,7 +3,9 @@ module Zeta.EAC
 open FStar.Seq
 open Zeta.SeqMachine
 open Zeta.Time
+open Zeta.Key
 open Zeta.App
+open Zeta.AppSimulate
 open Zeta.Record
 open Zeta.GenericVerifier
 open Zeta.High.Verifier
@@ -13,62 +15,83 @@ let evict_vlog_entry (app: app_params) = e:(vlog_entry app) {is_evict e}
 let nevict_vlog_entry (app: app_params) = e:(vlog_entry app) {not (is_evict e)}
 
 type vlog_entry_ext (app: app_params) =
-  | NEvict: e:vlog_entry app{not (is_evict e)} -> vlog_entry_ext app
+  | NEvict: e:vlog_entry app{is_internal e && not (is_evict e)} -> vlog_entry_ext app
   | EvictMerkle: e:vlog_entry app{is_merkle_evict e} -> v:value app -> vlog_entry_ext app
   | EvictBlum: e:vlog_entry app{is_blum_evict e} -> v:value app -> tid:thread_id -> vlog_entry_ext app
+  | App: e:vlog_entry app{is_appfn e} -> rs: seq (record app) -> vlog_entry_ext app
 
 let vlog_ext (app: app_params) = seq (vlog_entry_ext app)
 
-type eac_state (app: app_params) =
-  | EACFail: eac_state app
-  | EACInit: eac_state app
-  | EACInStore: m:add_method -> v:value app -> eac_state app
-  | EACEvictedMerkle: v:value app -> eac_state app
-  | EACEvictedBlum: v:value app -> t:timestamp -> j:thread_id -> eac_state app
-  | EACRoot: eac_state app
+type eac_state (app: app_params) (k: base_key) =
+  | EACFail: eac_state app k
+  | EACInit: eac_state app k
+  | EACInStore: m:add_method -> v:value app -> eac_state app k
+  | EACEvictedMerkle: v:value app -> eac_state app k
+  | EACEvictedBlum: v:value app -> t:timestamp -> j:thread_id -> eac_state app k
 
-let is_eac_state_evicted #app (s: eac_state app): bool =
+let is_eac_state_evicted #app #k (s: eac_state app k): bool =
   match s with
   | EACEvictedMerkle _ -> true
   | EACEvictedBlum _ _ _ -> true
   | _ -> false
 
-let is_eac_state_instore #app (s: eac_state app): bool =
+let is_eac_state_instore #app #k (s: eac_state app k): bool =
   match s with
   | EACInStore _ _ -> true
   | _ -> false
 
-let eac_add #app (e: vlog_entry_ext app) (s: eac_state app) : eac_state app
-  = match s with
-    | EACFail ->
-      EACFail
+let refs_key #app (e: vlog_entry app) (k: base_key)
+  = match e with
+    | AddM _ k' _ -> k' = k
+    | AddB _ k' _ _ -> k' = k
+    | EvictM k' _ -> k' = k
+    | EvictB k' _ -> k' = k
+    | EvictBM k' _ _ -> k' = k
+    | NextEpoch -> false
+    | VerifyEpoch -> false
+    | RunApp _ _ ks -> mem k ks
 
-    | EACInit -> (
-      match e with
+let to_vlog_entry #app (ee:vlog_entry_ext app): vlog_entry app =
+  match ee with
+  | EvictMerkle e _ -> e
+  | EvictBlum e _ _ -> e
+  | NEvict e -> e
+  | App e _ -> e
 
-      | NEvict (AddM (k,v) _ _) ->
-        if v = init_value k
-        then EACInStore MAdd v
-        else EACFail
-
-      | NEvict NextEpoch ->
-        EACRoot
-
-      | NEvict VerifyEpoch ->
-        EACRoot
-
-      | _ ->
+let eac_add #app #ks (ee: vlog_entry_ext app) (s: eac_state app ks) : eac_state app ks
+  = let e = to_vlog_entry ee in
+    (* if this entry does not reference key ks, the state is unchanged *)
+    if not (e `refs_key` ks) then s
+    else
+      match s with
+      | EACFail ->
         EACFail
-      )
+
+      | EACInit -> (
+        match ee with
+
+        | NEvict (AddM (k,v) _ _) ->
+          if v = init_value k then EACInStore MAdd v
+          else EACFail
+
+        | NEvict NextEpoch ->
+          s
+
+        | NEvict VerifyEpoch ->
+          s
+
+        | _ ->
+          EACFail
+        )
 
     | EACInStore m v -> (
-      match e with
+      match ee with
+      | App (RunApp f p _) rs ->
+        if length rs <> appfn_arity f then EACFail
+        else
+          EACFail
 
-      | NEvict (RunApp f p ss) ->
-        (* TODO fix this *)
-        EACFail
-
-      | EvictMerkle (EvictM _ _) v' ->
+      | EvictMerkle (EvictM  _ _) v' ->
         if AppV? v && v' <> v then EACFail
         else if IntV? v && not (IntV? v') then EACFail
         else EACEvictedMerkle v'
@@ -88,7 +111,7 @@ let eac_add #app (e: vlog_entry_ext app) (s: eac_state app) : eac_state app
     )
 
     | EACEvictedMerkle v -> (
-      match e with
+      match ee with
       | NEvict (AddM (_,v') _ _) ->
         if v' = v then EACInStore MAdd v
         else EACFail
@@ -96,41 +119,24 @@ let eac_add #app (e: vlog_entry_ext app) (s: eac_state app) : eac_state app
     )
 
     | EACEvictedBlum v t tid -> (
-      match e with
+      match ee with
       | NEvict (AddB (_,v') _ t' tid') ->
         if v' = v && t' = t && tid' = tid then EACInStore BAdd v
         else EACFail
       | _ -> EACFail
     )
 
-    | EACRoot -> (
-      match e with
-      | NEvict NextEpoch -> EACRoot
-      | NEvict VerifyEpoch -> EACRoot
-      | _ -> EACFail
-    )
-
-let eac_smk (app: app_params) = SeqMachine EACInit EACFail (eac_add #app)
-
-let to_vlog_entry #app (ee:vlog_entry_ext app): vlog_entry app =
-  match ee with
-  | EvictMerkle e _ -> e
-  | EvictBlum e _ _ -> e
-  | NEvict e -> e
-
-let vlog_entry_ext_key (e: vlog_entry_ext): key =
-  V.key_of (to_vlog_entry e)
-
-let eac_sm = PSM eac_smk vlog_entry_ext_key
+let eac_smk (app: app_params) (k: base_key) = SeqMachine EACInit EACFail (eac_add #app #k)
 
 (* evict add consistency *)
-let eac (l:vlog_ext) = valid_all eac_sm l
+let eac #app (l:vlog_ext app) =
+  forall (k: base_key). {:pattern Zeta.SeqMachine.valid (eac_smk app k) l} Zeta.SeqMachine.valid (eac_smk app k) l
 
 (* refinement of evict add consistent logs *)
-type eac_log = l:vlog_ext{eac l}
+let eac_log app = l:vlog_ext app{eac l}
 
-let is_eac_log (l:vlog_ext): (r:bool{r <==> eac l}) =
-  valid_all_comp eac_sm l
+(* computable version of eac *)
+val is_eac_log (#app: app_params) (l:vlog_ext app): (r:bool{r <==> eac l})
 
 let max_eac_prefix (l:vlog_ext{not (is_eac_log l)}):
   (i:nat{i < length l /\
